Wip

LeanVips/Asm/Basic.lean
@@ -32,21 +32,86 @@ inductive Instr where
   | j (imm26: Bv26) : Instr
 deriving Repr, Inhabited
 
--- Instruction shorthands
-@[match_pattern] def and  (rd rs rt: Reg) : Instr := .r .and rd rs rt
-@[match_pattern] def or   (rd rs rt: Reg) : Instr := .r .or  rd rs rt
-@[match_pattern] def add  (rd rs rt: Reg) : Instr := .r .add rd rs rt
-@[match_pattern] def sub  (rd rs rt: Reg) : Instr := .r .sub rd rs rt
-@[match_pattern] def slt  (rd rs rt: Reg) : Instr := .r .slt rd rs rt
-@[match_pattern] def andi (rt rs: Reg) (imm16: Bv16): Instr := .i .andi rt rs imm16
-@[match_pattern] def ori  (rt rs: Reg) (imm16: Bv16): Instr := .i .ori  rt rs imm16
-@[match_pattern] def addi (rt rs: Reg) (imm16: Bv16): Instr := .i .addi rt rs imm16
-@[match_pattern] def slti (rt rs: Reg) (imm16: Bv16): Instr := .i .slti rt rs imm16
-@[match_pattern] def lw   (rt rs: Reg) (imm16: Bv16): Instr := .i .lw   rt rs imm16
-@[match_pattern] def sw   (rt rs: Reg) (imm16: Bv16): Instr := .i .sw   rt rs imm16
-@[match_pattern] def beq  (rt rs: Reg) (imm16: Bv16): Instr := .i .beq  rt rs imm16
-@[match_pattern] def bne  (rt rs: Reg) (imm16: Bv16): Instr := .i .bne  rt rs imm16
+#check (Instr.i I.andi t0 t1 42)
+
+-- Instruction assembly shorthands
+@[match_pattern] def and  (rd rs rt: Reg) : Instr := .r .and rs rt rd
+@[match_pattern] def or   (rd rs rt: Reg) : Instr := .r .or  rs rt rd
+@[match_pattern] def add  (rd rs rt: Reg) : Instr := .r .add rs rt rd
+@[match_pattern] def sub  (rd rs rt: Reg) : Instr := .r .sub rs rt rd
+@[match_pattern] def slt  (rd rs rt: Reg) : Instr := .r .slt rs rt rd
+@[match_pattern] def andi (rt rs: Reg) (imm16: Bv16): Instr := .i .andi rs rt imm16
+@[match_pattern] def ori  (rt rs: Reg) (imm16: Bv16): Instr := .i .ori  rs rt imm16
+@[match_pattern] def addi (rt rs: Reg) (imm16: Bv16): Instr := .i .addi rs rt imm16
+@[match_pattern] def slti (rt rs: Reg) (imm16: Bv16): Instr := .i .slti rs rt imm16
+@[match_pattern] def lw   (rt rs: Reg) (imm16: Bv16): Instr := .i .lw   rs rt imm16
+@[match_pattern] def sw   (rt rs: Reg) (imm16: Bv16): Instr := .i .sw   rs rt imm16
+@[match_pattern] def beq  (rt rs: Reg) (imm16: Bv16): Instr := .i .beq  rs rt imm16
+@[match_pattern] def bne  (rt rs: Reg) (imm16: Bv16): Instr := .i .bne  rs rt imm16
 @[match_pattern] def j                 (imm26: Bv26): Instr := .j             imm26
+
+#check (andi t1 t1 42)
+
+theorem andi_equal: andi t1 t0 42 = Instr.i I.andi t0 t1 42 :=
+  by
+   simp [andi]
+
+theorem andi_equal_quant: ∀ (rs rt imm16), andi rt rs imm16 = Instr.i I.andi rs rt imm16 :=
+  by
+   simp [andi]
+
+theorem ori_equal_quant: ∀ (rs rt imm16), ori rt rs imm16 = Instr.i I.ori rs rt imm16 :=
+  by
+   simp [ori]
+
+theorem addi_equal_quant: ∀ (rs rt imm16), addi rt rs imm16 = Instr.i I.addi rs rt imm16 :=
+  by
+   simp [addi]
+
+theorem slti_equal_quant: ∀ (rs rt imm16), slti rt rs imm16 = Instr.i I.slti rs rt imm16 :=
+  by
+   simp [slti]
+
+theorem lw_equal_quant: ∀ (rs rt imm16), lw rt rs imm16 = Instr.i I.lw rs rt imm16 :=
+  by
+   simp [lw]
+
+theorem sw_equal_quant: ∀ (rs rt imm16), sw rt rs imm16 = Instr.i I.sw rs rt imm16 :=
+  by
+   simp [sw]
+
+theorem beq_equal_quant: ∀ (rs rt imm16), beq rt rs imm16 = Instr.i I.beq rs rt imm16 :=
+  by
+   simp [beq]
+
+theorem bne_equal_quant: ∀ (rs rt imm16), bne rt rs imm16 = Instr.i I.bne rs rt imm16 :=
+  by
+   simp [bne]
+
+theorem and_equal_quant: ∀ (rs rt rd), and rd rs rt = Instr.r R.and rs rt rd :=
+  by
+   simp [and]
+
+theorem or_equal_quant: ∀ (rs rt rd), or rd rs rt = Instr.r R.or rs rt rd :=
+  by
+   simp [or]
+
+theorem add_equal_quant: ∀ (rs rt rd), add rd rs rt = Instr.r R.add rs rt rd :=
+  by
+   simp [add]
+
+theorem sub_equal_quant: ∀ (rs rt rd), sub rd rs rt = Instr.r R.sub rs rt rd :=
+  by
+   simp [sub]
+
+theorem slt_equal_quant: ∀ (rs rt rd), slt rd rs rt = Instr.r R.slt rs rt rd :=
+  by
+   simp [slt]
+
+theorem j_equal_quant: ∀ (imm26), j imm26 = Instr.j imm26 :=
+  by
+   simp [j]
+
 
 -- Instruction memory
 abbrev IMem : Type := Array Instr
@@ -67,7 +132,7 @@ def DMem.r (dm: DMem) (addr: Bv32) : Bv32 :=
 -- Instruction evaluation semantics
 def instr_eval (instr: Instr) (pc: Bv32) (rf:Regfile) (dm: DMem):Regfile × DMem × Bv32 :=
   match instr  with
-  | .r op rd rs rt => -- R type instructions
+  | .r op rs rt rd => -- R type instructions
      let a := rf.r rs
      let b := rf.r rt
      (match op with
@@ -76,10 +141,10 @@ def instr_eval (instr: Instr) (pc: Bv32) (rf:Regfile) (dm: DMem):Regfile × DMem
      | .add => rf.w rd (a + b)
      | .sub => rf.w rd (a - b)
      | .slt => rf.w rd (if a < b then 1 else 0), dm, pc)
-  | .i .sw  rt rs imm16 => (rf, dm.w (rf.r rs + imm16.signExtend _) (rf.r rt), pc)
-  | .i .beq rt rs imm16 => (rf, dm, if rf.r rs == rf.r rt then pc + (imm16.signExtend _ <<< 2) else pc)
-  | .i .bne rt rs imm16 => (rf, dm, if rf.r rs != rf.r rt then pc + (imm16.signExtend _ <<< 2) else pc)
-  | .i op rt rs imm16 => -- I type instructions
+  | .i .sw  rs rt imm16 => (rf, dm.w (rf.r rs + imm16.signExtend _) (rf.r rt), pc)
+  | .i .beq rs rt imm16 => (rf, dm, if rf.r rs == rf.r rt then pc + (imm16.signExtend _ <<< 2) else pc)
+  | .i .bne rs rt imm16 => (rf, dm, if rf.r rs != rf.r rt then pc + (imm16.signExtend _ <<< 2) else pc)
+  | .i op rs rt imm16 => -- I type instructions
     let a := rf.r rs
     (match op with
     | .andi => rf.w rt (a &&& imm16.zeroExtend _)
