README.md
@@ -25,7 +25,7 @@ In the `Lean InfoView`should now see the current status (state) of Lean, reflect
 
 ### Evaluation
 
-Put your cursor at the end of line 99. 
+Put your cursor at the end of line 7. 
 
 ```lean
 #eval (toBv32 (and  t0 t1 t2)) [Cursor here] 
@@ -39,15 +39,15 @@ Basic.lean:99:0
 ```
 The `#32` indicate that the resulting value is a 32-bit bit vector (more on `BitVec` later). 
 
-You can try neighboring lines, and see the translation to binary for other instructions and/or change the `mnemonic` or operands (the rd, rs, rt arguments) to obtain the corresponding code. You can use this later for your lab5.
+You can try neighboring lines, and see the translation to binary for other instructions and/or change the *mnemonic* or *operands* (the *rd*, *rs*, *rt* arguments) to obtain the corresponding machine code. Hint, you can use this later for your lab5 programming exercise.
 
-Put your cursor at the end of line 381.
+Now, put your cursor at the end of line 36.
 
 ```lean
 #eval (eval imem 9 0x00 rf dm) [your cursor here]
 ```
 
-Lean will show the result of evaluating the `eval` definition (function), as three values, the first is the resulting register file (an array of 32 words), second is the data memory (dynamic array being empty in this case) and lastly the value of the `pc` register.
+Lean will show the result of evaluating the `eval` definition (function) as a tuple of three values `(RegisterFile,  DMem, Bv32)`. Fhe first `RegisterFile` is the resulting register file (an array of 32 words), second `DMem` is the data memory (dynamic array being empty in this case) and third and last, the value of the program counter register.
 
 Looking at the arguments of `eval imem 9 0x00 rf dm`. 
 - `imem`is the instruction memory definition (our program to execute)
@@ -62,11 +62,11 @@ Looking at the arguments of `eval imem 9 0x00 rf dm`.
   ori  t5 t3 0xFFFF  --20
   ```
 - `9`is the number of simulation steps we want to run (in this case 9).
-- `0x00`is the initial value for the `pc` register (the instruction memory starts at address 0).
-- `rf`is the initial state of the register file, declared at line 378 to be a vector of 32, 0 valued words.
-- `dm`is the initial state of the data memory, declared at line 379 as empty
+- `0x00`is the initial value for the `pc` register (the instruction memory starts at address 0x00).
+- `rf`is the initial state of the register file, declared at line 33 to be a vector of 32, 0 valued words.
+- `dm`is the initial state of the data memory, declared at line 34 as empty.
 
-The state after simulating 9 instructions is:
+The state after simulating 9 instructions is presented as the tuple:
 
 ```lean
 ({ toArray := #[0x00000000#32, 0x00000000#32, 0x00000000#32, 0x00000000#32, 0x00000000#32, 0x00000000#32, 0x00000000#32,
@@ -87,18 +87,152 @@ Now, you can try increase the number of instructions to simulate to 10.
 
 ```lean
 #eval (eval imem 10 0x00 rf dm) [your cursor here]
-
 ```
 
-This will result in an error (`index out of bounds`), as trying to read an instruction address outside of the defined instruction memory `imem`.
+This will result in an error (`index out of bounds`), as trying to read the instruction at address 0x24, which is outside of the defined instruction memory `imem`.
 
-Already now you can use `lean_vips`, as a way to write and simulate VIPS assembly programs, without knowing exactly how the modelling in Lean is done.
+Already now you can use `lean_vips`, as a way to write and simulate VIPS assembly programs, without knowing exactly how the modelling of the VIPS in Lean is implemented.
 
-Notice here, the complete definition of VIPS in Lean is less than 100 lines of code (the rest of the code is examples and proofs).
+Notice here, the complete definition of VIPS in Lean is less than 100 lines of code (the rest of the code is examples and proofs), Lean as a programming language allows for succint "lean" implementations.
 
 ## The VIPS model in Lean
 
-The 
+At hart of the model we define the data structures capturing the VIPS instruction set:
+
+```lean
+-- BitVectors
+abbrev Bv32:  Type := BitVec 32
+abbrev Bv16:  Type := BitVec 16
+abbrev Bv26:  Type := BitVec 26
+
+-- Registers
+abbrev Reg  : Type := BitVec 5
+
+-- Other fields
+abbrev Op   : Type := BitVec 6
+abbrev Funct: Type := BitVec 6
+abbrev Shamt: Type := BitVec 5
+
+inductive R where
+  | and : R
+  | or  : R
+  | add : R
+  | sub : R
+  | slt : R
+deriving Repr
+
+inductive I where
+  | andi : I
+  | ori  : I
+  | addi : I
+  | slti : I
+  | lw   : I
+  | sw   : I
+  | beq  : I
+  | bne  : I
+deriving Repr, BEq
+
+inductive Instr where
+  | i (instr: I) (rs rt: Reg) (imm: Bv16) : Instr
+  | r (instr: R) (rs rt rd: Reg) : Instr
+  | j (imm26: Bv26) : Instr
+deriving Repr, Inhabited
+```
+
+`Instr` here is the top level type, with three variants (constructors) `i`, `r`, and `j` to capture the three instruction classes.
+
+`Reg` is the type of registers where the `BitVec 5` type represents 5-bit values:
+
+```lean
+abbrev Reg  : Type := BitVec 5
+```
+
+Similarly, `Op`, `Funct` and `Shamt` fields are represented by `BitVector` types of corresponding width.
+
+The `Reg` definition along with constructors `zero, at', v0` etc., are given in the `LeanVips/Reg.Basic.lean`.
+
+Altogether the definitions now let us construct VIPS assembly instructions and check them, e.g.:
+
+```lean
+#check (Instr.i I.andi t0 t1 42) [place cursor here]
+``` 
+Will give you:
+```lean
+Instr.i I.andi t0 t1 42 : Instr
+```
+
+Here `t0` gives the `rs` field (one of the source operands), and `t1` the `rt` field (the destination for the `addi`). You can try constructing a few other instructions to get the hang of it.
+
+While possible to create machine code instructions, the syntax is inconvenient, so let us define some short-hands for assembly language input:
+
+```lean
+...
+@[match_pattern] def addi (rt rs: Reg) (imm16: Bv16): Instr := .i .addi rs rt imm16
+... 
+```
+
+You can now use these shorthands to construct VIPS assembly instructions, lets check this one: 
+
+```lean
+#check (andi t1 t0 42)
+```
+
+You should now have:
+```lean
+andi t1 t0 42 : Instr
+```
+
+Notice, here `Instr.i I.andi t0 t1 42 : Instr` and `andi t1 t0 42 : Instr`, are just two different ways to construct the exact same instruction. The `andi` constructor follows the assembly syntax with the `rt` (destination) field first, while the `Instr.i` constructor adheres to the machine level encoding of the fields.
+
+So can we show that they are the same? Let us try this!
+
+```lean
+theorem andi_equal: andi t1 t0 42 = Instr.i I.andi t0 t1 42 :=
+  by
+   simp [andi]
+```
+
+The theorem states the equality, and is solved (proven) by the `simp` tactic, using the definition of `andi`.
+
+As a sanity check, you may try introducing some error, e.g.:
+
+```lean
+theorem andi_equal: andi t1 t0 42 = Instr.i I.andi t0 t1 43 :=
+  by
+   simp [andi]
+```
+
+Now, the `by` gets *squiggled*, indicating that the attempted proof no longer holds (effectively 42 != 43).
+
+Similarly, we can try another error:
+
+```lean
+theorem andi_equal: andi t1 t0 42 = Instr.i I.andi t1 t0 42 :=
+  by
+   simp [andi]
+```
+
+Also here the proof attempt fails, in this case due to the order of register operands.
+
+To gain further confidence, we can generalize over all possible rs, rt and immediate assignments.
+
+```lean
+theorem andi_equal_quant: ∀ (rs rt imm16), andi rt rs imm16 = Instr.i I.andi rs rt imm16 :=
+  by
+   simp [andi]
+```
+
+With the current encoding is however harder to further generalize (showing that this holds for all the shorthands defined). Instead we show it case by case for each supported instruction. (Room for future improvement, in case larger subset of instructions should be supported.)
+
+
+
+
+
+
+
+
+The VIPS model is a subset of the MIPS32 ISA, refer to [MIPS Greencard](https://booksite.elsevier.com/9780124077263/downloads/COD_5e_Greencard.pdf) for the complete MIPS32 instruction set.
+
 
 
 
